update defs and proofs for weak bisim

abs0_abs1_thm/abs_weak_bisimulationScript.sml
@@ -1,42 +1,65 @@
 open HolKernel bossLib boolLib Parse;
-open SPI_stateTheory;
+open SPI_stateTheory weak_bisimulationTheory;
 open ds_abs0_relTheory abs_relTheory;
 open ds_abs1_relTheory;
-open abs_rel_holds_call_lblTheory;
+open abs_rel_holds_abs1_tau_spiTheory abs_rel_holds_abs1_tau_drTheory abs_rel_holds_abs1_tau_combTheory abs_rel_holds_call_lblTheory abs_rel_holds_TX_lblTheory abs_rel_holds_RX_lblTheory abs_rel_holds_XFER_lblTheory abs_rel_holds_abs0_tauTheory;
 
 val _ = new_theory "abs_weak_bisimulation";
 
-1.define weak transition relation
-weak R s1 lbl s2 = (s1 = s2 /\ lbl = tau) \/
-R s1 lbl s2 \/ 
-(?s3. s1 tau s3 /\ weak R s3 lbl s2)
+(*
+val f_def = Define `
+f a = (T \/ (f a))`
+*)
 
-2.define weak-bisim 
-weak-bisim B R 
-!s1 s2. B s1 s2 ==> !lbl s3. weak R s1 lbl s3 ==> ?s4. weak R s2 lbl s4 /\ B s3 s4 /\
-!lbl s4. weak R s2 lbl s4 ==> ?s3. weak R s1 lbl s3 /\ B s3 s4
+(* a state can be reached after n tau steps 
+val n_tau_tr_def = Define `
+(n_tau_tr (0:num) (tr:'a -> global_lbl_type -> 'a -> bool) (s:'a) (lbl:global_lbl_type) (s':'a) = (tr s lbl s')) /\
+(n_tau_tr (n:num) (tr:'a -> global_lbl_type -> 'a -> bool) (s:'a) (lbl:global_lbl_type) (s':'a) = ?(s'':'a). (tr s tau s'') /\ (n_tau_tr (n-1) tr s'' lbl s'))`
 
+(* define the weak transition relation *)
+val weak_tr_def = Define `
+weak_tr (tr:'a -> global_lbl_type -> 'a -> bool) (s:'a) (lbl:global_lbl_type) (s':'a) = 
+((tr s lbl s') \/
+(s = s' /\ lbl = tau) \/
+(?n. n_tau_tr n tr s lbl s'))`
 
-(* weak bisimulation between ds_abs0 and ds_abs1 *)
-(* have to rewrite *)
-val abs0_weak_bisimulation = store_thm("abs0_weak_bisimulation",
+(* define the weak bisimulation realtion *)
+val weak_bisim_def = Define `
+weak_bisim (r:'a -> 'b -> bool) (tr1:'a -> global_lbl_type -> 'a -> bool) (tr2:'b -> global_lbl_type -> 'b -> bool) =
+(!s1 s2. r s1 s2 ==>
+(!lbl s1'. tr1 s1 lbl s1' ==> ?s2'. weak_tr tr2 s2 lbl s2' /\ r s1' s2') /\
+(!lbl s2'. tr2 s2 lbl s2' ==> ?s1'. weak_tr tr1 s1 lbl s1' /\ r s1' s2'))`
+*)
+
+val abs0_weak_simulation = store_thm("abs0_weak_simulation",
 ``!ds_abs0 ds_abs1 lbl ds_abs0'.
 (abs_rel ds_abs0 ds_abs1) /\ (ds_abs0_tr ds_abs0 lbl ds_abs0') ==>
-?ds_abs1'. (tau_linked_lbl ds_abs1 ds_abs1' lbl) /\ (abs_rel ds_abs1' ds_abs0')``,
-rw [ds_abs0_tr_cases] >>
+(?ds_abs1'.(ds_abs1_tr ds_abs1 lbl ds_abs1') /\ (abs_rel ds_abs0' ds_abs1')) \/
+(?n ds_abs1'. (n_tau_tr n ds_abs1_tr ds_abs1 lbl ds_abs1') /\ (abs_rel ds_abs0' ds_abs1'))``,
+rw [ds_abs0_tr_cases] >> 
 rw [abs0_abs_rel_call_init, abs0_abs_rel_call_tx, abs0_abs_rel_call_rx,
-abs0_abs_rel_call_xfer] >>
-cheat);
+abs0_abs_rel_call_xfer, abs_rel_holds_abs_tau, abs_rel_holds_abs0_TX_lbl, 
+abs_rel_holds_abs0_RX_lbl, abs_rel_holds_abs0_XFER_lbl]
+(* TO PROVE: TX labels *));
 
-
-val abs1_weak_bisimulation = store_thm("abs1_weak_bisimulation",
+val abs1_weak_simulation = store_thm("abs1_weak_simulation",
 ``!ds_abs0 ds_abs1 lbl ds_abs1'.
 (abs_rel ds_abs0 ds_abs1) /\ (ds_abs1_tr ds_abs1 lbl ds_abs1') ==>
+(lbl = tau ==> 
 (abs_rel ds_abs0 ds_abs1') \/
-(?ds_abs0'. (ds_abs0_tr ds_abs0 lbl ds_abs0') /\ (abs_rel ds_abs0' ds_abs1'))``,
-rw [ds_abs1_tr_cases] >>
+(?ds_abs0'. (ds_abs0_tr ds_abs0 lbl ds_abs0') /\ (abs_rel ds_abs0' ds_abs1'))) /\
+(lbl <> tau ==> 
+?ds_abs0'. (ds_abs0_tr ds_abs0 lbl ds_abs0') /\ (abs_rel ds_abs0' ds_abs1'))``,
+rw [ds_abs1_tr_cases] >> 
 rw [abs1_init_pre_abs_rel_call_init, abs1_ready_abs_rel_call_init, 
-abs1_abs_rel_call_tx, abs1_abs_rel_call_rx, abs1_abs_rel_call_xfer] >>
-cheat);
+abs1_abs_rel_call_tx, abs1_abs_rel_call_rx, abs1_abs_rel_call_xfer,
+abs_rel_holds_abs1_TX_lbl, abs_rel_holds_abs1_RX_lbl, abs_rel_holds_abs1_XFER_lbl] >>
+METIS_TAC [abs_rel_holds_abs1_tau_spi, abs_rel_holds_abs1_tau_dr, 
+abs_rel_holds_abs1_tau_comb]);
+
+val weak_bisim_abs0_abs1 = store_thm("weak_bisim_abs0_abs1",
+``weak_bisim abs_rel ds_abs0_tr ds_abs1_tr``,
+rw [weak_bisim_def, weak_tr_def] >>
+METIS_TAC [abs0_weak_simulation, abs1_weak_simulation]);
 
 val _ = export_theory();
