abs0_abs1_thm/abs_rel_holds_RX_lblScript.sml
@@ -1,0 +1,72 @@
+open HolKernel bossLib boolLib Parse;
+open SPI_stateTheory ds_abs1_stateTheory weak_bisimulationTheory;
+open ds_abs0_relTheory abs_relTheory ds_abs0_rxTheory;
+open ds_abs1_relTheory ds_abs1_rxTheory;
+
+val _ = new_theory "abs_rel_holds_RX_lbl";
+
+(* abs_rel holds when ds_abs1 peforms RX label transition *)
+val abs_rel_holds_abs1_RX_lbl = store_thm("abs_rel_holds_abs1_RX_lbl",
+``!(ds_abs0:ds_abs0_state) (ds_abs1:ds_abs1_state) (data: word8 option).
+(abs_rel ds_abs0 ds_abs1) /\ (ABS1_RX_LBL_ENABLE ds_abs1) /\ (data <> NONE) ==>
+?ds_abs0'. ds_abs0_tr ds_abs0 (RX data) ds_abs0' /\ 
+abs_rel ds_abs0' (abs1_rx_receive_data_op ds_abs1 data)``,
+rw [ABS1_RX_LBL_ENABLE_def] >>
+`IS_ABS_STATE_REL ds_abs0 ds_abs1` by METIS_TAC [abs_rel_def] >|
+[(* abs1_rx_receive *)
+`ds_abs0.state = abs0_rx_idle` by METIS_TAC [IS_ABS_STATE_REL_def] >>
+rw [ds_abs0_tr_cases, ABS0_RX_LBL_ENABLE_def, abs0_rx_op_def, 
+abs1_rx_receive_data_op_def, abs0_rx_idle_op_def, abs1_rx_receive_op_def] >>
+fs [abs_rel_def, IS_ABS_STATE_REL_def],
+(* abs1_rx_fetch_data *)
+`ds_abs0.state = abs0_rx_reading` by METIS_TAC [IS_ABS_STATE_REL_def] >>
+rw [ds_abs0_tr_cases, ABS0_RX_LBL_ENABLE_def, abs0_rx_op_def, 
+abs1_rx_receive_data_op_def, abs0_rx_reading_op_def, abs1_rx_fetch_data_op_def] >>
+fs [abs_rel_def, IS_ABS_STATE_REL_def]]);
+
+(* abs_rel holds when ds_abs0 peforms RX label transition *)
+val abs_rel_holds_abs0_RX_lbl = store_thm("abs_rel_holds_abs0_RX_lbl",
+``!(ds_abs0:ds_abs0_state) (ds_abs1:ds_abs1_state) (data: word8 option).
+(abs_rel ds_abs0 ds_abs1) /\ (ABS0_RX_LBL_ENABLE ds_abs0) /\ (data <> NONE) ==>
+(?ds_abs1'. ds_abs1_tr ds_abs1 (RX data) ds_abs1' /\
+abs_rel (abs0_rx_op ds_abs0 data) ds_abs1')\/
+(?n ds_abs1'. n_tau_tr n ds_abs1_tr ds_abs1 (RX data) ds_abs1' /\
+abs_rel (abs0_rx_op ds_abs0 data) ds_abs1')``,
+rw [ABS0_RX_LBL_ENABLE_def] >>
+`IS_ABS_STATE_REL ds_abs0 ds_abs1` by METIS_TAC [abs_rel_def] >|
+[(* abs0_rx_idle *)
+rw [abs0_rx_op_def, abs0_rx_idle_op_def] >>
+`ds_abs1.state = abs1_rx_receive \/ ds_abs1.state = abs1_rx_idle` 
+by METIS_TAC [IS_ABS_STATE_REL_def] >|
+[(* abs1_rx_receive *)
+DISJ1_TAC >>
+rw [ds_abs1_tr_cases, ABS1_RX_LBL_ENABLE_def, abs1_rx_receive_data_op_def, abs1_rx_receive_op_def] >>
+fs [abs_rel_def, IS_ABS_STATE_REL_def],
+(* abs1_rx_idle *)
+DISJ2_TAC >>
+EXISTS_TAC ``SUC 0:num`` >>
+rw [n_tau_tr_def, ds_abs1_tr_cases, ds_abs1_spi_tr_cases, SPI_ABS1_RX_ENABLE_def, 
+GSYM LEFT_EXISTS_AND_THM] >>
+EXISTS_TAC ``spi_abs1_rx_operations ds_abs1`` >>
+rw [spi_abs1_rx_operations_def, spi_abs1_rx_idle_op_def, ABS1_RX_LBL_ENABLE_def, 
+abs1_rx_receive_data_op_def, abs1_rx_receive_op_def] >>
+fs [abs_rel_def, IS_ABS_STATE_REL_def]],
+(* abs1_rx_reading *)
+rw [abs0_rx_op_def, abs0_rx_reading_op_def] >>
+`ds_abs1.state = abs1_rx_fetch_data \/ ds_abs1.state = abs1_rx_read` 
+by METIS_TAC [IS_ABS_STATE_REL_def] >|
+[(* abs1_rx_fetch_data *)
+DISJ1_TAC >>
+rw [ds_abs1_tr_cases, ABS1_RX_LBL_ENABLE_def, abs1_rx_receive_data_op_def, abs1_rx_fetch_data_op_def] >>
+fs [abs_rel_def, IS_ABS_STATE_REL_def],
+(* abs1_rx_read *)
+DISJ2_TAC >>
+EXISTS_TAC ``SUC 0:num`` >>
+rw [n_tau_tr_def, ds_abs1_tr_cases, ds_abs1_comb_tr_cases, COMB_ABS1_RX_ENABLE_def,
+GSYM LEFT_EXISTS_AND_THM] >>
+EXISTS_TAC ``comb_abs1_rx_operations ds_abs1`` >>
+rw [comb_abs1_rx_operations_def, comb_abs1_rx_read_op_def, ABS1_RX_LBL_ENABLE_def,
+abs1_rx_receive_data_op_def, abs1_rx_fetch_data_op_def] >>
+fs [abs_rel_def, IS_ABS_STATE_REL_def]]]);
+
+val _ = export_theory();
