abs0_abs1_thm/abs_rel_holds_TX_lblScript.sml
@@ -1,0 +1,61 @@
+open HolKernel bossLib boolLib Parse;
+open SPI_stateTheory ds_abs1_stateTheory;
+open ds_abs0_relTheory abs_relTheory ds_abs0_txTheory;
+open ds_abs1_relTheory ds_abs1_txTheory;
+
+val _ = new_theory "abs_rel_holds_TX_lbl";
+
+(* abs_rel holds when ds_abs1 peforms TX label transition *)
+val abs_rel_holds_abs1_TX_lbl = store_thm("abs_rel_holds_abs1_TX_lbl",
+``!(ds_abs0:ds_abs0_state) (ds_abs1:ds_abs1_state).
+(abs_rel ds_abs0 ds_abs1) /\ (ABS1_TX_LBL_ENABLE ds_abs1) ==>
+?ds_abs0'. ds_abs0_tr ds_abs0 (TX (abs1_tx_trans_done_op_value ds_abs1)) ds_abs0' /\ 
+abs_rel ds_abs0' (abs1_tx_trans_done_op_state ds_abs1)``,
+rw [ABS1_TX_LBL_ENABLE_def, abs1_tx_trans_done_op_state_def, 
+abs1_tx_trans_done_op_value_def, abs1_tx_trans_done_op_def] >>
+`IS_ABS_STATE_REL ds_abs0 ds_abs1` by METIS_TAC [abs_rel_def] >>
+`ds_abs0.state = abs0_tx` by METIS_TAC [IS_ABS_STATE_REL_def] >|
+[(* abs1_tx_done_1 *)
+`ds_abs1.ds_abs1_tx.tx_cur_length = ds_abs0.ds_abs0_tx.tx_cur_length + 1` by METIS_TAC [abs_rel_def] >>
+`~ (ds_abs1.ds_abs1_tx.tx_cur_length < LENGTH ds_abs1.ds_abs1_tx.tx_data_buffer)` by METIS_TAC [abs_rel_def] >>
+`ds_abs1.ds_abs1_tx.tx_data_buffer = ds_abs0.ds_abs0_tx.tx_data_buffer` by METIS_TAC [abs_rel_def] >>
+`~ (ds_abs0.ds_abs0_tx.tx_cur_length < LENGTH ds_abs0.ds_abs0_tx.tx_data_buffer - 1)` by fs [] >>
+rw [ds_abs0_tr_cases, abs0_tx_op_value_def, abs0_tx_op_state_def, abs0_tx_op_def] >|
+[fs [abs_rel_def],
+fs [abs_rel_def, IS_ABS_STATE_REL_def]],
+(* abs1_tx_done_2 *)
+`ds_abs1.ds_abs1_tx.tx_cur_length = ds_abs0.ds_abs0_tx.tx_cur_length + 1` by METIS_TAC [abs_rel_def] >>
+`ds_abs1.ds_abs1_tx.tx_cur_length < LENGTH ds_abs1.ds_abs1_tx.tx_data_buffer` by METIS_TAC [abs_rel_def] >>
+`ds_abs1.ds_abs1_tx.tx_data_buffer = ds_abs0.ds_abs0_tx.tx_data_buffer` by METIS_TAC [abs_rel_def] >>
+`ds_abs0.ds_abs0_tx.tx_cur_length < LENGTH ds_abs0.ds_abs0_tx.tx_data_buffer - 1` by fs [] >>
+rw [ds_abs0_tr_cases, abs0_tx_op_value_def, abs0_tx_op_state_def, abs0_tx_op_def] >|
+[fs [abs_rel_def],
+fs [abs_rel_def, IS_ABS_STATE_REL_def]],
+(* abs1_tx_next *)
+`ds_abs1.ds_abs1_tx.tx_cur_length = ds_abs0.ds_abs0_tx.tx_cur_length + 2` by METIS_TAC [abs_rel_def] >>
+`ds_abs1.ds_abs1_tx.tx_cur_length < LENGTH ds_abs1.ds_abs1_tx.tx_data_buffer` by METIS_TAC [abs_rel_def] >>
+`ds_abs1.ds_abs1_tx.tx_data_buffer = ds_abs0.ds_abs0_tx.tx_data_buffer` by METIS_TAC [abs_rel_def] >>
+`ds_abs0.ds_abs0_tx.tx_cur_length < LENGTH ds_abs0.ds_abs0_tx.tx_data_buffer - 1` by fs [] >>
+rw [ds_abs0_tr_cases, abs0_tx_op_value_def, abs0_tx_op_state_def, abs0_tx_op_def] >|
+[fs [abs_rel_def],
+fs [abs_rel_def, IS_ABS_STATE_REL_def]],
+(* abs1_tx_last *)
+`ds_abs1.ds_abs1_tx.tx_cur_length = ds_abs0.ds_abs0_tx.tx_cur_length + 2` by METIS_TAC [abs_rel_def] >>
+`ds_abs1.ds_abs1_tx.tx_cur_length = LENGTH ds_abs1.ds_abs1_tx.tx_data_buffer` by METIS_TAC [abs_rel_def] >>
+`ds_abs1.ds_abs1_tx.tx_data_buffer = ds_abs0.ds_abs0_tx.tx_data_buffer` by METIS_TAC [abs_rel_def] >>
+`ds_abs0.ds_abs0_tx.tx_cur_length < LENGTH ds_abs0.ds_abs0_tx.tx_data_buffer - 1` by fs [] >>
+rw [ds_abs0_tr_cases, abs0_tx_op_value_def, abs0_tx_op_state_def, abs0_tx_op_def] >|
+[fs [abs_rel_def],
+fs [abs_rel_def, IS_ABS_STATE_REL_def]]]);
+
+(* abs_rel holds when ds_abs0 peforms TX label transition *)
+val abs_rel_holds_abs0_TX_lbl = store_thm("abs_rel_holds_abs0_TX_lbl",
+``!(ds_abs0:ds_abs0_state) (ds_abs1:ds_abs1_state).
+(abs_rel ds_abs0 ds_abs1) /\ (ds_abs0.state = abs0_tx) ==>
+(?ds_abs1'. ds_abs1_tr ds_abs1 (TX (abs0_tx_op_value ds_abs0)) ds_abs1' /\ 
+abs_rel (abs0_tx_op_state ds_abs0) ds_abs1') \/
+(?n ds_abs1'. n_tau_tr n ds_abs1_tr ds_abs1 (TX (abs0_tx_op_value ds_abs0)) ds_abs1' /\
+abs_rel (abs0_tx_op_state ds_abs0) ds_abs1')``,
+cheat);
+
+val _ = export_theory();
