abs0_abs1_thm/abs_rel_holds_abs0_tauScript.sml
@@ -1,0 +1,193 @@
+open HolKernel bossLib boolLib Parse;
+open SPI_stateTheory ds_abs1_stateTheory weak_bisimulationTheory;
+open ds_abs0_relTheory abs_relTheory ds_abs0_tauTheory ds_abs0_rxTheory ds_abs0_xferTheory;
+open ds_abs1_relTheory ds_abs1_initTheory ds_abs1_txTheory ds_abs1_rxTheory ds_abs1_xferTheory;
+
+val _ = new_theory "abs_rel_holds_abs0_tau";
+
+(* a lemma for n_tau_tr *)
+val n_tau_tr_SUC = store_thm("n_tau_tr_SUC",
+``!tr s s' n lbl. (n > 0) ==> 
+n_tau_tr n tr s lbl s' = n_tau_tr (SUC (n - 1)) tr s lbl s'``, 
+rw [] >>
+`n = SUC (n - 1)` by  fs[] >>
+METIS_TAC[]);
+
+(* abs_rel holds when ds_abs0.state = abs0_rx_update *)
+val abs_rel_holds_tau_abs0_rx_update = store_thm("abs_rel_holds_tau_abs0_rx_update",
+``!(ds_abs0:ds_abs0_state) (ds_abs1:ds_abs1_state).
+(abs_rel ds_abs0 ds_abs1) /\ (ds_abs0.state = abs0_rx_update) ==>
+(?ds_abs1'. ds_abs1_tr ds_abs1 tau ds_abs1' /\ abs_rel (abs0_tau_op ds_abs0) ds_abs1') \/
+(?n ds_abs1'. n_tau_tr n ds_abs1_tr ds_abs1 tau ds_abs1' /\ abs_rel (abs0_tau_op ds_abs0) ds_abs1')``,
+rw [abs0_tau_op_def, abs0_rx_update_tau_op_def] >>
+`IS_ABS_STATE_REL ds_abs0 ds_abs1` by METIS_TAC [abs_rel_def] >>
+`ds_abs1.state = abs1_rx_ready \/ ds_abs1.state = abs1_rx_update` by METIS_TAC [IS_ABS_STATE_REL_def] >|
+[(* rx_left_length > 0, abs1_rx_ready *)
+`ds_abs1.ds_abs1_rx.rx_left_length > 0` by METIS_TAC [abs_rel_def] >>
+DISJ1_TAC >>
+rw [ds_abs1_tr_cases, ds_abs1_dr_tr_cases, DRIVER_ABS1_RX_ENABLE_def] >>
+EXISTS_TAC ``driver_abs1_rx_operations ds_abs1`` >>
+rw [driver_abs1_rx_operations_def, driver_abs1_rx_ready_op_def] >>
+fs [abs_rel_def, IS_ABS_STATE_REL_def],
+(* rx_left_length > 0, abs1_rx_update *)
+DISJ2_TAC >>
+EXISTS_TAC ``SUC 0:num`` >>
+rw [n_tau_tr_def, ds_abs1_tr_cases, ds_abs1_spi_tr_cases, SPI_ABS1_RX_ENABLE_def, 
+ds_abs1_dr_tr_cases, GSYM LEFT_EXISTS_AND_THM] >>
+EXISTS_TAC ``driver_abs1_rx_operations (spi_abs1_rx_operations ds_abs1)`` >>
+EXISTS_TAC ``spi_abs1_rx_operations ds_abs1`` >>
+`ds_abs1.ds_abs1_rx.rx_left_length > 0` by METIS_TAC [abs_rel_def] >>
+rw [spi_abs1_rx_operations_def, spi_abs1_rx_update_op_def, 
+driver_abs1_rx_operations_def, driver_abs1_rx_ready_op_def, DRIVER_ABS1_RX_ENABLE_def] >>
+fs [abs_rel_def, IS_ABS_STATE_REL_def],
+(* rx_left_length <= 0, abs1_rx_ready *)
+`~ (ds_abs1.ds_abs1_rx.rx_left_length > 0)` by METIS_TAC [abs_rel_def] >>
+DISJ1_TAC >>
+rw [ds_abs1_tr_cases, ds_abs1_dr_tr_cases, DRIVER_ABS1_RX_ENABLE_def] >>
+EXISTS_TAC ``driver_abs1_rx_operations ds_abs1`` >>
+rw [driver_abs1_rx_operations_def, driver_abs1_rx_ready_op_def] >>
+fs [abs_rel_def, IS_ABS_STATE_REL_def],
+(* rx_left_length <= 0, abs1_rx_update *)
+DISJ2_TAC >>
+EXISTS_TAC ``SUC 0:num`` >>
+rw [n_tau_tr_def, ds_abs1_tr_cases, ds_abs1_spi_tr_cases, SPI_ABS1_RX_ENABLE_def, 
+ds_abs1_dr_tr_cases, GSYM LEFT_EXISTS_AND_THM] >>
+EXISTS_TAC ``driver_abs1_rx_operations (spi_abs1_rx_operations ds_abs1)`` >>
+EXISTS_TAC ``spi_abs1_rx_operations ds_abs1`` >>
+`~(ds_abs1.ds_abs1_rx.rx_left_length > 0)` by METIS_TAC [abs_rel_def] >>
+rw [spi_abs1_rx_operations_def, spi_abs1_rx_update_op_def, 
+driver_abs1_rx_operations_def, driver_abs1_rx_ready_op_def, DRIVER_ABS1_RX_ENABLE_def] >>
+fs [abs_rel_def, IS_ABS_STATE_REL_def]]);
+
+(* abs_rel holds when ds_abs0.state = abs0_rx_reading *)
+val abs_rel_holds_tau_abs0_rx_reading = store_thm("abs_rel_holds_tau_abs0_rx_reading",
+``!(ds_abs0:ds_abs0_state) (ds_abs1:ds_abs1_state).
+(abs_rel ds_abs0 ds_abs1) /\ (ds_abs0.state = abs0_rx_reading) ==>
+(?ds_abs1'. ds_abs1_tr ds_abs1 tau ds_abs1' /\ abs_rel (abs0_tau_op ds_abs0) ds_abs1') \/
+(?n ds_abs1'. n_tau_tr n ds_abs1_tr ds_abs1 tau ds_abs1' /\ abs_rel (abs0_tau_op ds_abs0) ds_abs1')``,
+rw [abs0_tau_op_def, abs0_rx_reading_tau_op_def] >>
+`IS_ABS_STATE_REL ds_abs0 ds_abs1` by METIS_TAC [abs_rel_def] >>
+`ds_abs1.state = abs1_rx_read \/ ds_abs1.state = abs1_rx_fetch_data` 
+by METIS_TAC [IS_ABS_STATE_REL_def] >|
+[(* abs1_rx_read *)
+DISJ2_TAC >>
+EXISTS_TAC ``SUC 0:num`` >>
+rw [n_tau_tr_def, ds_abs1_tr_cases, ds_abs1_comb_tr_cases, ds_abs1_dr_tr_cases,
+COMB_ABS1_RX_ENABLE_def, GSYM LEFT_EXISTS_AND_THM] >>
+EXISTS_TAC ``driver_abs1_rx_operations (comb_abs1_rx_operations ds_abs1)`` >>
+EXISTS_TAC ``comb_abs1_rx_operations ds_abs1`` >>
+rw [comb_abs1_rx_operations_def, comb_abs1_rx_read_op_def,
+driver_abs1_rx_operations_def, driver_abs1_rx_fetch_data_op_def, DRIVER_ABS1_RX_ENABLE_def] >>
+fs [abs_rel_def, IS_ABS_STATE_REL_def],
+DISJ1_TAC >>
+rw [ds_abs1_tr_cases, ds_abs1_dr_tr_cases, DRIVER_ABS1_RX_ENABLE_def] >>
+EXISTS_TAC ``driver_abs1_rx_operations ds_abs1`` >>
+rw [driver_abs1_rx_operations_def, driver_abs1_rx_fetch_data_op_def] >>
+fs [abs_rel_def, IS_ABS_STATE_REL_def]]);
+
+(* abs_rel holds when ds_abs0.state = abs0_rx_next *)
+val abs_rel_holds_tau_abs0_rx_next = store_thm("abs_rel_holds_tau_abs0_rx_next",
+``!(ds_abs0:ds_abs0_state) (ds_abs1:ds_abs1_state).
+(abs_rel ds_abs0 ds_abs1) /\ (ds_abs0.state = abs0_rx_next) ==>
+?ds_abs1'. ds_abs1_tr ds_abs1 tau ds_abs1' /\ abs_rel (abs0_tau_op ds_abs0) ds_abs1'``,
+rw [abs0_tau_op_def, abs0_rx_next_tau_op_def] >>
+`IS_ABS_STATE_REL ds_abs0 ds_abs1` by METIS_TAC [abs_rel_def] >>
+`ds_abs1.state = abs1_rx_next \/ ds_abs1.state = abs1_rx_next_ready` 
+by METIS_TAC [IS_ABS_STATE_REL_def] >>
+rw [ds_abs1_tr_cases, ds_abs1_dr_tr_cases, DRIVER_ABS1_RX_ENABLE_def] >>
+EXISTS_TAC ``driver_abs1_rx_operations ds_abs1`` >>
+rw [driver_abs1_rx_operations_def, driver_abs1_rx_next_op_def, driver_abs1_rx_next_ready_op_def] >>
+fs [abs_rel_def, IS_ABS_STATE_REL_def]);
+
+(* abs_rel_holds when ds_abs0.state = abs0_xfer_done *)
+val abs_rel_holds_tau_abs0_xfer_done = store_thm("abs_rel_holds_tau_abs0_xfer_done",
+``!(ds_abs0:ds_abs0_state) (ds_abs1:ds_abs1_state).
+(abs_rel ds_abs0 ds_abs1) /\ (ds_abs0.state = abs0_xfer_done) ==>
+(?ds_abs1'. ds_abs1_tr ds_abs1 tau ds_abs1' /\ abs_rel (abs0_tau_op ds_abs0) ds_abs1') \/
+(?n ds_abs1'. n_tau_tr n ds_abs1_tr ds_abs1 tau ds_abs1' /\ abs_rel (abs0_tau_op ds_abs0) ds_abs1')``,
+rw [abs0_tau_op_def, abs0_xfer_tau_op_def] >>
+`IS_ABS_STATE_REL ds_abs0 ds_abs1` by METIS_TAC [abs_rel_def] >>
+`ds_abs1.state = abs1_xfer_fetch_data \/ ds_abs1.state = abs1_xfer_ready \/
+ds_abs1.state = abs1_xfer_update` by METIS_TAC [IS_ABS_STATE_REL_def] >>
+`ds_abs0.ds_abs0_xfer.xfer_cur_length = ds_abs1.ds_abs1_xfer.xfer_cur_length` by fs [abs_rel_def] >|
+[(* not the last one, abs1_xfer_fetch_data *)
+DISJ1_TAC >>
+`ds_abs1.ds_abs1_xfer.xfer_cur_length < LENGTH ds_abs1.ds_abs1_xfer.xfer_dataOUT_buffer` 
+by METIS_TAC [abs_rel_def] >>
+rw [ds_abs1_tr_cases, ds_abs1_dr_tr_cases, DRIVER_ABS1_XFER_ENABLE_def] >>
+EXISTS_TAC ``driver_abs1_xfer_operations ds_abs1`` >> 
+rw [driver_abs1_xfer_operations_def, driver_abs1_xfer_fetch_data_op_def] >>
+fs [abs_rel_def, IS_ABS_STATE_REL_def],
+(* not the last one, abs1_xfer_ready *)
+DISJ2_TAC >>
+`ds_abs1.ds_abs1_xfer.xfer_cur_length < LENGTH ds_abs1.ds_abs1_xfer.xfer_dataOUT_buffer` 
+by METIS_TAC [abs_rel_def] >>
+EXISTS_TAC ``SUC 0: num`` >>
+rw [n_tau_tr_def, ds_abs1_tr_cases, ds_abs1_comb_tr_cases, ds_abs1_dr_tr_cases,
+COMB_ABS1_XFER_ENABLE_def, GSYM LEFT_EXISTS_AND_THM] >>
+EXISTS_TAC ``driver_abs1_xfer_operations (comb_abs1_xfer_operations ds_abs1)`` >>
+EXISTS_TAC ``comb_abs1_xfer_operations ds_abs1`` >>
+rw [comb_abs1_xfer_operations_def, comb_abs1_xfer_ready_op_def, DRIVER_ABS1_XFER_ENABLE_def, 
+driver_abs1_xfer_operations_def, driver_abs1_xfer_fetch_data_op_def] >>
+fs [abs_rel_def, IS_ABS_STATE_REL_def],
+(* not the last one, abs1_xfer_update *)
+DISJ2_TAC >>
+`ds_abs1.ds_abs1_xfer.xfer_cur_length < LENGTH ds_abs1.ds_abs1_xfer.xfer_dataOUT_buffer` 
+by METIS_TAC [abs_rel_def] >>
+EXISTS_TAC ``SUC 1:num`` >>
+rw [n_tau_tr_def, n_tau_tr_SUC, GSYM LEFT_EXISTS_AND_THM, GSYM RIGHT_EXISTS_AND_THM] >>
+EXISTS_TAC ``driver_abs1_xfer_operations (comb_abs1_xfer_operations (spi_abs1_xfer_operations ds_abs1)) `` >>
+EXISTS_TAC ``spi_abs1_xfer_operations ds_abs1`` >>
+EXISTS_TAC ``comb_abs1_xfer_operations (spi_abs1_xfer_operations ds_abs1)`` >>
+rw [ds_abs1_tr_cases, ds_abs1_spi_tr_cases, ds_abs1_comb_tr_cases, ds_abs1_dr_tr_cases,
+COMB_ABS1_XFER_ENABLE_def, SPI_ABS1_XFER_ENABLE_def, DRIVER_ABS1_XFER_ENABLE_def,
+spi_abs1_xfer_operations_def, spi_abs1_xfer_update_op_def, comb_abs1_xfer_operations_def,
+comb_abs1_xfer_ready_op_def, driver_abs1_xfer_operations_def, driver_abs1_xfer_fetch_data_op_def] >>
+fs [abs_rel_def, IS_ABS_STATE_REL_def],
+(* last one, abs1_xfer_fetch_data *)
+DISJ1_TAC >>
+`~ (ds_abs1.ds_abs1_xfer.xfer_cur_length < LENGTH ds_abs1.ds_abs1_xfer.xfer_dataOUT_buffer)` 
+by METIS_TAC [abs_rel_def] >>
+rw [ds_abs1_tr_cases, ds_abs1_dr_tr_cases, DRIVER_ABS1_XFER_ENABLE_def] >>
+EXISTS_TAC ``driver_abs1_xfer_operations ds_abs1`` >> 
+rw [driver_abs1_xfer_operations_def, driver_abs1_xfer_fetch_data_op_def] >>
+fs [abs_rel_def, IS_ABS_STATE_REL_def],
+(* last one, abs1_xfer_done *)
+DISJ2_TAC >>
+`~ (ds_abs1.ds_abs1_xfer.xfer_cur_length < LENGTH ds_abs1.ds_abs1_xfer.xfer_dataOUT_buffer)` 
+by METIS_TAC [abs_rel_def] >>
+EXISTS_TAC ``SUC 0: num`` >>
+rw [n_tau_tr_def, ds_abs1_tr_cases, ds_abs1_comb_tr_cases, ds_abs1_dr_tr_cases,
+COMB_ABS1_XFER_ENABLE_def, GSYM LEFT_EXISTS_AND_THM] >>
+EXISTS_TAC ``driver_abs1_xfer_operations (comb_abs1_xfer_operations ds_abs1)`` >>
+EXISTS_TAC ``comb_abs1_xfer_operations ds_abs1`` >>
+rw [comb_abs1_xfer_operations_def, comb_abs1_xfer_ready_op_def, DRIVER_ABS1_XFER_ENABLE_def, 
+driver_abs1_xfer_operations_def, driver_abs1_xfer_fetch_data_op_def] >>
+fs [abs_rel_def, IS_ABS_STATE_REL_def],
+(* last one, abs1_xfer_update *)
+DISJ2_TAC >>
+`~ (ds_abs1.ds_abs1_xfer.xfer_cur_length < LENGTH ds_abs1.ds_abs1_xfer.xfer_dataOUT_buffer)` 
+by METIS_TAC [abs_rel_def] >>
+EXISTS_TAC ``SUC 1:num`` >>
+rw [n_tau_tr_def, n_tau_tr_SUC, GSYM LEFT_EXISTS_AND_THM, GSYM RIGHT_EXISTS_AND_THM] >>
+EXISTS_TAC ``driver_abs1_xfer_operations (comb_abs1_xfer_operations (spi_abs1_xfer_operations ds_abs1)) `` >>
+EXISTS_TAC ``spi_abs1_xfer_operations ds_abs1`` >>
+EXISTS_TAC ``comb_abs1_xfer_operations (spi_abs1_xfer_operations ds_abs1)`` >>
+rw [ds_abs1_tr_cases, ds_abs1_spi_tr_cases, ds_abs1_comb_tr_cases, ds_abs1_dr_tr_cases,
+COMB_ABS1_XFER_ENABLE_def, SPI_ABS1_XFER_ENABLE_def, DRIVER_ABS1_XFER_ENABLE_def,
+spi_abs1_xfer_operations_def, spi_abs1_xfer_update_op_def, comb_abs1_xfer_operations_def,
+comb_abs1_xfer_ready_op_def, driver_abs1_xfer_operations_def, driver_abs1_xfer_fetch_data_op_def] >>
+fs [abs_rel_def, IS_ABS_STATE_REL_def]]);
+
+(* abs_rel holds when ds_abs0 peforms tau transitions *)
+val abs_rel_holds_abs0_tau = store_thm("abs_rel_holds_abs_tau",
+``!(ds_abs0:ds_abs0_state) (ds_abs1:ds_abs1_state).
+(abs_rel ds_abs0 ds_abs1) /\ (ABS0_TAU_LBL_ENABLE ds_abs0) ==>
+(?ds_abs1'. ds_abs1_tr ds_abs1 tau ds_abs1' /\ abs_rel (abs0_tau_op ds_abs0) ds_abs1') \/
+(?n ds_abs1'. n_tau_tr n ds_abs1_tr ds_abs1 tau ds_abs1' /\ abs_rel (abs0_tau_op ds_abs0) ds_abs1')``,
+rw [ABS0_TAU_LBL_ENABLE_def] >>
+rw [abs_rel_holds_tau_abs0_rx_update, abs_rel_holds_tau_abs0_rx_reading,
+abs_rel_holds_tau_abs0_rx_next, abs_rel_holds_tau_abs0_xfer_done]);
+
+
+val _ = export_theory();
