abs0_abs1_thm/abs_rel_holds_abs1_tau_combScript.sml
@@ -20,7 +20,11 @@ val abs_rel_holds_abs1_tau_comb_tx = store_thm("abs_rel_holds_abs1_tau_comb_tx",
 (abs_rel ds_abs0 (comb_abs1_tx_operations ds_abs1))``,
 rw [COMB_ABS1_TX_ENABLE_def, comb_abs1_tx_operations_def] >>
 rw [comb_abs1_tx_trans_op_def, comb_abs1_tx_done_2_op_def, comb_abs1_tx_reset_op_def] >>
-fs [abs_rel_def, IS_ABS_STATE_REL_def] >> cheat);
+fs [abs_rel_def, IS_ABS_STATE_REL_def] >> 
+`ds_abs1.ds_abs1_tx.tx_cur_length = ds_abs0.ds_abs0_tx.tx_cur_length + 1` by fs [] >|
+[fs[],
+`ds_abs1.ds_abs1_tx.tx_cur_length < LENGTH ds_abs1.ds_abs1_tx.tx_data_buffer` by fs [] >>
+fs[]]);
 
 (* abs_rel holds for ds_abs1 tau_comb in the rx automaton *)
 val abs_rel_holds_abs1_tau_comb_rx = store_thm("abs_rel_holds_abs1_tau_comb_rx",
@@ -39,7 +43,7 @@ val abs_rel_holds_abs1_tau_comb_xfer = store_thm("abs_rel_holds_abs1_tau_comb_xf
 rw [COMB_ABS1_XFER_ENABLE_def, comb_abs1_xfer_operations_def] >>
 rw [comb_abs1_xfer_prepare_op_def, comb_abs1_xfer_ready_op_def, 
 comb_abs1_xfer_reset_op_def] >>
-fs [abs_rel_def, IS_ABS_STATE_REL_def] >> cheat);
+fs [abs_rel_def, IS_ABS_STATE_REL_def]);
 
 (* abs_rel holds when ds_abs1 peforms tau_comb *)
 val abs_rel_holds_abs1_tau_comb = store_thm("abs_rel_holds_abs1_tau_comb",
