abs0_abs1_thm/abs_rel_holds_abs1_tau_drScript.sml
@@ -17,25 +17,25 @@ rw [DRIVER_ABS1_RX_ENABLE_def, driver_abs1_rx_operations_def] >>
 `ds_abs0.state = abs0_rx_update` by METIS_TAC [IS_ABS_STATE_REL_def] >>
 rw [driver_abs1_rx_ready_op_def] >|
 [`ds_abs0.ds_abs0_rx.rx_left_length > 0` by METIS_TAC [abs_rel_def] >>
-rw [ds_abs0_tr_cases, ABS0_TAU_LBL_ENABLE_def, abs0_tau_op_def, abs0_rx_update_op_def] >>
+rw [ds_abs0_tr_cases, ABS0_TAU_LBL_ENABLE_def, abs0_tau_op_def, abs0_rx_update_tau_op_def] >>
 fs [abs_rel_def, IS_ABS_STATE_REL_def],
 `~(ds_abs0.ds_abs0_rx.rx_left_length > 0)` by METIS_TAC [abs_rel_def] >>
-rw [ds_abs0_tr_cases, ABS0_TAU_LBL_ENABLE_def, abs0_tau_op_def, abs0_rx_update_op_def] >>
+rw [ds_abs0_tr_cases, ABS0_TAU_LBL_ENABLE_def, abs0_tau_op_def, abs0_rx_update_tau_op_def] >>
 fs [abs_rel_def, IS_ABS_STATE_REL_def]],
 (* abs1_rx_fetch_data *)
 `ds_abs0.state = abs0_rx_reading` by METIS_TAC [IS_ABS_STATE_REL_def] >>
 rw [driver_abs1_rx_fetch_data_op_def] >>
-rw [ds_abs0_tr_cases, ABS0_TAU_LBL_ENABLE_def, abs0_tau_op_def, abs0_rx_reading_op_def] >>
+rw [ds_abs0_tr_cases, ABS0_TAU_LBL_ENABLE_def, abs0_tau_op_def, abs0_rx_reading_tau_op_def] >>
 fs [abs_rel_def, IS_ABS_STATE_REL_def],
 (* abs1_rx_next *)
 `ds_abs0.state = abs0_rx_next` by METIS_TAC [IS_ABS_STATE_REL_def] >>
 rw [driver_abs1_rx_next_op_def] >>
-rw [ds_abs0_tr_cases, ABS0_TAU_LBL_ENABLE_def, abs0_tau_op_def, abs0_rx_next_op_def] >>
+rw [ds_abs0_tr_cases, ABS0_TAU_LBL_ENABLE_def, abs0_tau_op_def, abs0_rx_next_tau_op_def] >>
 fs [abs_rel_def, IS_ABS_STATE_REL_def],
 (* abs1_rx_next_ready *)
 `ds_abs0.state = abs0_rx_next` by METIS_TAC [IS_ABS_STATE_REL_def] >>
 rw [driver_abs1_rx_next_ready_op_def] >>
-rw [ds_abs0_tr_cases, ABS0_TAU_LBL_ENABLE_def, abs0_tau_op_def, abs0_rx_next_op_def] >>
+rw [ds_abs0_tr_cases, ABS0_TAU_LBL_ENABLE_def, abs0_tau_op_def, abs0_rx_next_tau_op_def] >>
 fs [abs_rel_def, IS_ABS_STATE_REL_def]]);
 
 (* abs_rel_holds for abs1 xfer automaton tau_dr transition *)
@@ -47,9 +47,11 @@ abs_rel ds_abs0' (driver_abs1_xfer_operations ds_abs1)``,
 rw [DRIVER_ABS1_XFER_ENABLE_def, driver_abs1_xfer_operations_def, driver_abs1_xfer_fetch_data_op_def] >>
 `IS_ABS_STATE_REL ds_abs0 ds_abs1` by METIS_TAC [abs_rel_def] >>
 `ds_abs0.state = abs0_xfer_done` by METIS_TAC [IS_ABS_STATE_REL_def] >|
-[`ds_abs0.ds_abs0_xfer.xfer_cur_length < LENGTH ds_abs0.ds_abs0_xfer.xfer_dataOUT_buffer` by METIS_TAC [abs_rel_def] >>
+[`ds_abs1.state <> abs1_xfer_data /\ ds_abs1.state <> abs1_xfer_exchange` by rw [] >>
+`ds_abs0.ds_abs0_xfer.xfer_cur_length < LENGTH ds_abs0.ds_abs0_xfer.xfer_dataOUT_buffer` by METIS_TAC [abs_rel_def] >>
 rw [ds_abs0_tr_cases, ABS0_TAU_LBL_ENABLE_def, abs0_tau_op_def, abs0_xfer_tau_op_def] >>
 fs [abs_rel_def, IS_ABS_STATE_REL_def],
+`ds_abs1.state <> abs1_xfer_data /\ ds_abs1.state <> abs1_xfer_exchange` by rw [] >>
 `~ (ds_abs0.ds_abs0_xfer.xfer_cur_length < LENGTH ds_abs0.ds_abs0_xfer.xfer_dataOUT_buffer)` by METIS_TAC [abs_rel_def] >>
 rw [ds_abs0_tr_cases, ABS0_TAU_LBL_ENABLE_def, abs0_tau_op_def, abs0_xfer_tau_op_def] >>
 fs [abs_rel_def, IS_ABS_STATE_REL_def]]);
