abs0_abs1_thm/abs_rel_holds_call_lblScript.sml
@@ -1,48 +1,62 @@
 open HolKernel bossLib boolLib Parse;
-open SPI_stateTheory;
+open SPI_stateTheory weak_bisimulationTheory;
 open ds_abs0_relTheory abs_relTheory ds_abs0_initTheory ds_abs0_txTheory ds_abs0_rxTheory ds_abs0_xferTheory;
 open ds_abs1_relTheory ds_abs1_initTheory ds_abs1_txTheory ds_abs1_rxTheory ds_abs1_xferTheory;
 
 val _ = new_theory "abs_rel_holds_call_lbl";
 
+(* Theorems for abs0_weak_simulation with call_label *)
 (* abs_rel holds for call_init label when ds_abs0 has call_init transition *)
 val abs0_abs_rel_call_init = store_thm("abs0_abs_rel_call_init",
 ``!ds_abs0 ds_abs1 ds_abs0'.
 (abs_rel ds_abs0 ds_abs1) /\ (ABS0_CALL_INIT_ENABLE ds_abs0) ==>
-?ds_abs1'. (ds_abs1_abs_tr ds_abs1 call_init ds_abs1') /\ 
-(abs_rel (call_init_ds_abs0 ds_abs0) ds_abs1')``,
+(?ds_abs1'. (ds_abs1_tr ds_abs1 call_init ds_abs1') /\ 
+(abs_rel (call_init_ds_abs0 ds_abs0) ds_abs1')) \/ 
+(?n ds_abs1'. n_tau_tr n ds_abs1_tr ds_abs1 call_init ds_abs1' /\ abs_rel (call_init_ds_abs0 ds_abs0) ds_abs1')``,
 rw [ABS0_CALL_INIT_ENABLE_def, call_init_ds_abs0_def] >>
 `IS_ABS_STATE_REL ds_abs0 ds_abs1` by METIS_TAC [abs_rel_def] >|
 [(* ds_abs0.state = abs0_init *)
+DISJ1_TAC >>
 `ds_abs1.state = abs1_init_pre` by METIS_TAC [IS_ABS_STATE_REL_def] >>
-rw [ds_abs1_abs_tr_cases, ds_abs1_tr_cases] >>
-EXISTS_TAC ``call_init_ds_abs1 ds_abs1`` >>
-rw [call_init_ds_abs1_def] >>
+rw [ds_abs1_tr_cases, call_init_ds_abs1_def] >>
 fs [abs_rel_def, IS_ABS_STATE_REL_def],
 (* ds_abs0.state = abs0_ready *)
 `ds_abs1.state = abs1_ready \/ ds_abs1.state = abs1_init_start \/
  ds_abs1.state = abs1_tx_reset \/ ds_abs1.state = abs1_rx_reset \/
- ds_abs1.state = abs1_xfer_reset` by METIS_TAC [IS_ABS_STATE_REL_def] >>
-rw [ds_abs1_abs_tr_cases, ds_abs1_tr_cases, ds_abs1_comb_tr_cases, 
-COMB_ABS1_INIT_ENABLE_def, COMB_ABS1_TX_ENABLE_def, COMB_ABS1_RX_ENABLE_def,
-COMB_ABS1_XFER_ENABLE_def, GSYM LEFT_EXISTS_AND_THM] >|
+ ds_abs1.state = abs1_xfer_reset` by METIS_TAC [IS_ABS_STATE_REL_def] >|
 [(* ds_abs1.state = abs1_ready *)
-EXISTS_TAC ``call_init_ds_abs1 ds_abs1`` >>
-rw [call_init_ds_abs1_def] >>
+DISJ1_TAC >>
+rw [ds_abs1_tr_cases, call_init_ds_abs1_def] >>
 fs [abs_rel_def, IS_ABS_STATE_REL_def],
 (* ds_abs1.state = abs1_init_start *)
+DISJ2_TAC >>
+EXISTS_TAC ``SUC 0:num`` >>
+rw [n_tau_tr_def, ds_abs1_tr_cases, ds_abs1_comb_tr_cases,
+COMB_ABS1_INIT_ENABLE_def, GSYM LEFT_EXISTS_AND_THM] >>
 EXISTS_TAC ``comb_abs1_init_operations ds_abs1`` >>
 rw [comb_abs1_init_operations_def, comb_abs1_init_start_op_def, call_init_ds_abs1_def] >>
 fs [abs_rel_def, IS_ABS_STATE_REL_def],
 (* ds_abs1.state = abs1_tx_reset *)
+DISJ2_TAC >>
+EXISTS_TAC ``SUC 0:num`` >>
+rw [n_tau_tr_def, ds_abs1_tr_cases, ds_abs1_comb_tr_cases, 
+COMB_ABS1_TX_ENABLE_def, GSYM LEFT_EXISTS_AND_THM] >>
 EXISTS_TAC ``comb_abs1_tx_operations ds_abs1`` >>
 rw [comb_abs1_tx_operations_def, comb_abs1_tx_reset_op_def, call_init_ds_abs1_def] >>
 fs [abs_rel_def, IS_ABS_STATE_REL_def],
 (* ds_abs1.state = abs1_rx_reset *)
+DISJ2_TAC >>
+EXISTS_TAC ``SUC 0:num`` >>
+rw [n_tau_tr_def, ds_abs1_tr_cases, ds_abs1_comb_tr_cases, 
+COMB_ABS1_RX_ENABLE_def, GSYM LEFT_EXISTS_AND_THM] >>
 EXISTS_TAC ``comb_abs1_rx_operations ds_abs1`` >>
 rw [comb_abs1_rx_operations_def, comb_abs1_rx_reset_op_def, call_init_ds_abs1_def] >>
 fs [abs_rel_def, IS_ABS_STATE_REL_def],
 (* ds_abs1.state = abs1_xfer_reset *)
+DISJ2_TAC >>
+EXISTS_TAC ``SUC 0:num`` >>
+rw [n_tau_tr_def, ds_abs1_tr_cases, ds_abs1_comb_tr_cases, 
+COMB_ABS1_XFER_ENABLE_def, GSYM LEFT_EXISTS_AND_THM] >>
 EXISTS_TAC ``comb_abs1_xfer_operations ds_abs1`` >>
 rw [comb_abs1_xfer_operations_def, comb_abs1_xfer_reset_op_def, call_init_ds_abs1_def] >>
 fs [abs_rel_def, IS_ABS_STATE_REL_def]]]);
@@ -51,33 +65,48 @@ fs [abs_rel_def, IS_ABS_STATE_REL_def]]]);
 val abs0_abs_rel_call_tx = store_thm("abs0_abs_rel_call_tx",
 ``!ds_abs0 ds_abs1 buffer.
 (abs_rel ds_abs0 ds_abs1) /\ (ds_abs0.state = abs0_ready) /\ (buffer <> []) ==>
-?ds_abs1'. (ds_abs1_abs_tr ds_abs1 (call_tx buffer) ds_abs1') /\ 
-(abs_rel (call_tx_ds_abs0 ds_abs0 buffer) ds_abs1')``,
+(?ds_abs1'. (ds_abs1_tr ds_abs1 (call_tx buffer) ds_abs1') /\ 
+(abs_rel (call_tx_ds_abs0 ds_abs0 buffer) ds_abs1')) \/ 
+(?n ds_abs1'. n_tau_tr n ds_abs1_tr ds_abs1 (call_tx buffer) ds_abs1' /\ 
+abs_rel (call_tx_ds_abs0 ds_abs0 buffer) ds_abs1')``,
 rw [call_tx_ds_abs0_def] >>
 `IS_ABS_STATE_REL ds_abs0 ds_abs1` by METIS_TAC [abs_rel_def] >>
 `ds_abs1.state = abs1_ready \/ ds_abs1.state = abs1_init_start \/
  ds_abs1.state = abs1_tx_reset \/ ds_abs1.state = abs1_rx_reset \/
- ds_abs1.state = abs1_xfer_reset` by METIS_TAC [IS_ABS_STATE_REL_def] >>
-rw [ds_abs1_abs_tr_cases, ds_abs1_tr_cases, ds_abs1_comb_tr_cases, 
-COMB_ABS1_INIT_ENABLE_def, COMB_ABS1_TX_ENABLE_def, COMB_ABS1_RX_ENABLE_def,
-COMB_ABS1_XFER_ENABLE_def, GSYM LEFT_EXISTS_AND_THM] >|
+ ds_abs1.state = abs1_xfer_reset` by METIS_TAC [IS_ABS_STATE_REL_def] >|
 [(* ds_abs1.state = abs1_ready *)
-EXISTS_TAC ``call_tx_ds_abs1 ds_abs1 buffer`` >>
-rw [call_tx_ds_abs1_def] >>
+DISJ1_TAC >>
+rw [ds_abs1_tr_cases, call_tx_ds_abs1_def] >>
 fs [abs_rel_def, IS_ABS_STATE_REL_def],
 (* ds_abs1.state = abs1_init_start *)
+DISJ2_TAC >>
+EXISTS_TAC ``SUC 0:num`` >>
+rw [n_tau_tr_def, ds_abs1_tr_cases, ds_abs1_comb_tr_cases,
+COMB_ABS1_INIT_ENABLE_def, GSYM LEFT_EXISTS_AND_THM] >>
 EXISTS_TAC ``comb_abs1_init_operations ds_abs1`` >>
 rw [comb_abs1_init_operations_def, comb_abs1_init_start_op_def, call_tx_ds_abs1_def] >>
 fs [abs_rel_def, IS_ABS_STATE_REL_def],
 (* ds_abs1.state = abs1_tx_reset *)
+DISJ2_TAC >>
+EXISTS_TAC ``SUC 0:num`` >>
+rw [n_tau_tr_def, ds_abs1_tr_cases, ds_abs1_comb_tr_cases, 
+COMB_ABS1_TX_ENABLE_def, GSYM LEFT_EXISTS_AND_THM] >>
 EXISTS_TAC ``comb_abs1_tx_operations ds_abs1`` >>
 rw [comb_abs1_tx_operations_def, comb_abs1_tx_reset_op_def, call_tx_ds_abs1_def] >>
 fs [abs_rel_def, IS_ABS_STATE_REL_def],
 (* ds_abs1.state = abs1_rx_reset *)
+DISJ2_TAC >>
+EXISTS_TAC ``SUC 0:num`` >>
+rw [n_tau_tr_def, ds_abs1_tr_cases, ds_abs1_comb_tr_cases, 
+COMB_ABS1_RX_ENABLE_def, GSYM LEFT_EXISTS_AND_THM] >>
 EXISTS_TAC ``comb_abs1_rx_operations ds_abs1`` >>
 rw [comb_abs1_rx_operations_def, comb_abs1_rx_reset_op_def, call_tx_ds_abs1_def] >>
 fs [abs_rel_def, IS_ABS_STATE_REL_def],
 (* ds_abs1.state = abs1_xfer_reset *)
+DISJ2_TAC >>
+EXISTS_TAC ``SUC 0:num`` >>
+rw [n_tau_tr_def, ds_abs1_tr_cases, ds_abs1_comb_tr_cases, 
+COMB_ABS1_XFER_ENABLE_def, GSYM LEFT_EXISTS_AND_THM] >>
 EXISTS_TAC ``comb_abs1_xfer_operations ds_abs1`` >>
 rw [comb_abs1_xfer_operations_def, comb_abs1_xfer_reset_op_def, call_tx_ds_abs1_def] >>
 fs [abs_rel_def, IS_ABS_STATE_REL_def]]);
@@ -86,33 +115,48 @@ fs [abs_rel_def, IS_ABS_STATE_REL_def]]);
 val abs0_abs_rel_call_rx = store_thm("abs0_abs_rel_call_rx",
 ``!ds_abs0 ds_abs1 length.
 (abs_rel ds_abs0 ds_abs1) /\ (ds_abs0.state = abs0_ready) /\ (length > 0) ==>
-?ds_abs1'. (ds_abs1_abs_tr ds_abs1 (call_rx length) ds_abs1') /\
-(abs_rel (call_rx_ds_abs0 ds_abs0 length) ds_abs1')``,
+(?ds_abs1'. (ds_abs1_tr ds_abs1 (call_rx length) ds_abs1') /\
+(abs_rel (call_rx_ds_abs0 ds_abs0 length) ds_abs1')) \/
+(?n ds_abs1'. n_tau_tr n ds_abs1_tr ds_abs1 (call_rx length) ds_abs1' /\
+abs_rel (call_rx_ds_abs0 ds_abs0 length) ds_abs1')``,
 rw [call_rx_ds_abs0_def] >>
 `IS_ABS_STATE_REL ds_abs0 ds_abs1` by METIS_TAC [abs_rel_def] >>
 `ds_abs1.state = abs1_ready \/ ds_abs1.state = abs1_init_start \/
  ds_abs1.state = abs1_tx_reset \/ ds_abs1.state = abs1_rx_reset \/
- ds_abs1.state = abs1_xfer_reset` by METIS_TAC [IS_ABS_STATE_REL_def] >>
-rw [ds_abs1_abs_tr_cases, ds_abs1_tr_cases, ds_abs1_comb_tr_cases, 
-COMB_ABS1_INIT_ENABLE_def, COMB_ABS1_TX_ENABLE_def, COMB_ABS1_RX_ENABLE_def,
-COMB_ABS1_XFER_ENABLE_def, GSYM LEFT_EXISTS_AND_THM] >|
+ ds_abs1.state = abs1_xfer_reset` by METIS_TAC [IS_ABS_STATE_REL_def] >|
 [(* abs1_ready *)
-EXISTS_TAC ``call_rx_ds_abs1 ds_abs1 length`` >>
-rw [call_rx_ds_abs1_def] >>
+DISJ1_TAC >>
+rw [ds_abs1_tr_cases, call_rx_ds_abs1_def] >>
 fs [abs_rel_def, IS_ABS_STATE_REL_def],
 (* abs1_init_start *)
+DISJ2_TAC >>
+EXISTS_TAC ``SUC 0:num`` >>
+rw [n_tau_tr_def, ds_abs1_tr_cases, ds_abs1_comb_tr_cases,
+COMB_ABS1_INIT_ENABLE_def, GSYM LEFT_EXISTS_AND_THM] >>
 EXISTS_TAC ``comb_abs1_init_operations ds_abs1`` >>
 rw [comb_abs1_init_operations_def, comb_abs1_init_start_op_def, call_rx_ds_abs1_def] >>
 fs [abs_rel_def, IS_ABS_STATE_REL_def],
 (* abs1_tx_reset *)
+DISJ2_TAC >>
+EXISTS_TAC ``SUC 0:num`` >>
+rw [n_tau_tr_def, ds_abs1_tr_cases, ds_abs1_comb_tr_cases, 
+COMB_ABS1_TX_ENABLE_def, GSYM LEFT_EXISTS_AND_THM] >>
 EXISTS_TAC ``comb_abs1_tx_operations ds_abs1`` >>
 rw [comb_abs1_tx_operations_def, comb_abs1_tx_reset_op_def, call_rx_ds_abs1_def] >>
 fs [abs_rel_def, IS_ABS_STATE_REL_def],
 (* abs1_rx_reset *)
+DISJ2_TAC >>
+EXISTS_TAC ``SUC 0:num`` >>
+rw [n_tau_tr_def, ds_abs1_tr_cases, ds_abs1_comb_tr_cases, 
+COMB_ABS1_RX_ENABLE_def, GSYM LEFT_EXISTS_AND_THM] >>
 EXISTS_TAC ``comb_abs1_rx_operations ds_abs1`` >>
 rw [comb_abs1_rx_operations_def, comb_abs1_rx_reset_op_def, call_rx_ds_abs1_def] >>
 fs [abs_rel_def, IS_ABS_STATE_REL_def],
 (* abs1_xfer_reset *)
+DISJ2_TAC >>
+EXISTS_TAC ``SUC 0:num`` >>
+rw [n_tau_tr_def, ds_abs1_tr_cases, ds_abs1_comb_tr_cases, 
+COMB_ABS1_XFER_ENABLE_def, GSYM LEFT_EXISTS_AND_THM] >>
 EXISTS_TAC ``comb_abs1_xfer_operations ds_abs1`` >>
 rw [comb_abs1_xfer_operations_def, comb_abs1_xfer_reset_op_def, call_rx_ds_abs1_def] >>
 fs [abs_rel_def, IS_ABS_STATE_REL_def]]);
@@ -121,37 +165,53 @@ fs [abs_rel_def, IS_ABS_STATE_REL_def]]);
 val abs0_abs_rel_call_xfer = store_thm("abs0_abs_rel_call_xfer",
 ``!ds_abs0 ds_abs1 buffer.
 (abs_rel ds_abs0 ds_abs1) /\ (ds_abs0.state = abs0_ready) /\ (buffer <> []) ==>
-?ds_abs1'. (ds_abs1_abs_tr ds_abs1 (call_xfer buffer) ds_abs1') /\ 
-(abs_rel (call_xfer_ds_abs0 ds_abs0 buffer) ds_abs1')``,
+(?ds_abs1'. (ds_abs1_tr ds_abs1 (call_xfer buffer) ds_abs1') /\ 
+(abs_rel (call_xfer_ds_abs0 ds_abs0 buffer) ds_abs1')) \/
+(?n ds_abs1'. n_tau_tr n ds_abs1_tr ds_abs1 (call_xfer buffer) ds_abs1' /\
+abs_rel (call_xfer_ds_abs0 ds_abs0 buffer) ds_abs1')``,
 rw [call_xfer_ds_abs0_def] >>
 `IS_ABS_STATE_REL ds_abs0 ds_abs1` by METIS_TAC [abs_rel_def] >>
 `ds_abs1.state = abs1_ready \/ ds_abs1.state = abs1_init_start \/
  ds_abs1.state = abs1_tx_reset \/ ds_abs1.state = abs1_rx_reset \/
- ds_abs1.state = abs1_xfer_reset` by METIS_TAC [IS_ABS_STATE_REL_def] >>
-rw [ds_abs1_abs_tr_cases, ds_abs1_tr_cases, ds_abs1_comb_tr_cases, 
-COMB_ABS1_INIT_ENABLE_def, COMB_ABS1_TX_ENABLE_def, COMB_ABS1_RX_ENABLE_def,
-COMB_ABS1_XFER_ENABLE_def, GSYM LEFT_EXISTS_AND_THM] >|
+ ds_abs1.state = abs1_xfer_reset` by METIS_TAC [IS_ABS_STATE_REL_def] >|
 [(* abs1_ready *)
-EXISTS_TAC ``call_xfer_ds_abs1 ds_abs1 buffer`` >>
-rw [call_xfer_ds_abs1_def] >>
+DISJ1_TAC >>
+rw [ds_abs1_tr_cases, call_xfer_ds_abs1_def] >>
 fs [abs_rel_def, IS_ABS_STATE_REL_def],
 (* abs1_init_start *)
+DISJ2_TAC >>
+EXISTS_TAC ``SUC 0:num`` >>
+rw [n_tau_tr_def, ds_abs1_tr_cases, ds_abs1_comb_tr_cases,
+COMB_ABS1_INIT_ENABLE_def, GSYM LEFT_EXISTS_AND_THM] >>
 EXISTS_TAC ``comb_abs1_init_operations ds_abs1`` >>
 rw [comb_abs1_init_operations_def, comb_abs1_init_start_op_def, call_xfer_ds_abs1_def] >>
 fs [abs_rel_def, IS_ABS_STATE_REL_def],
 (* abs1_tx_reset *)
+DISJ2_TAC >>
+EXISTS_TAC ``SUC 0:num`` >>
+rw [n_tau_tr_def, ds_abs1_tr_cases, ds_abs1_comb_tr_cases, 
+COMB_ABS1_TX_ENABLE_def, GSYM LEFT_EXISTS_AND_THM] >>
 EXISTS_TAC ``comb_abs1_tx_operations ds_abs1`` >>
 rw [comb_abs1_tx_operations_def, comb_abs1_tx_reset_op_def, call_xfer_ds_abs1_def] >>
 fs [abs_rel_def, IS_ABS_STATE_REL_def],
 (* abs1_rx_reset *)
+DISJ2_TAC >>
+EXISTS_TAC ``SUC 0:num`` >>
+rw [n_tau_tr_def, ds_abs1_tr_cases, ds_abs1_comb_tr_cases, 
+COMB_ABS1_RX_ENABLE_def, GSYM LEFT_EXISTS_AND_THM] >>
 EXISTS_TAC ``comb_abs1_rx_operations ds_abs1`` >>
 rw [comb_abs1_rx_operations_def, comb_abs1_rx_reset_op_def, call_xfer_ds_abs1_def] >>
 fs [abs_rel_def, IS_ABS_STATE_REL_def],
 (* abs1_xfer_reset *)
+DISJ2_TAC >>
+EXISTS_TAC ``SUC 0:num`` >>
+rw [n_tau_tr_def, ds_abs1_tr_cases, ds_abs1_comb_tr_cases, 
+COMB_ABS1_XFER_ENABLE_def, GSYM LEFT_EXISTS_AND_THM] >>
 EXISTS_TAC ``comb_abs1_xfer_operations ds_abs1`` >>
 rw [comb_abs1_xfer_operations_def, comb_abs1_xfer_reset_op_def, call_xfer_ds_abs1_def] >>
 fs [abs_rel_def, IS_ABS_STATE_REL_def]]);
 
+(* Theorems for abs1_weak_simulation with call labels *)
 (* abs_rel holds for call_init label when ds_abs1 state is abs1_init_pre *)
 val abs1_init_pre_abs_rel_call_init = store_thm("abs1_init_pre_abs_rel_call_init",
 ``!ds_abs0 ds_abs1.
