abs1_comb_thm/abs1_comb_simulationScript.sml
@@ -15,7 +15,7 @@ val _ = new_theory "abs1_comb_simulation";
 
 (* simulation: ds_abs1' exists when lbl is not tau *)
 val abs1_comb_hold_ref_rel_not_tau_lbl = store_thm("abs1_comb_hold_ref_rel_not_tau_lbl",
-``!(spi:spi_state) (dr:driver_state) (ds_abs1:ds_abs1_state) (lbl:global_lbl_type).
+``!(spi:spi_state) (dr:driver_state) (ds_abs1:ds_abs1_state) (lbl:global_lbl_type) (dr':driver_state) (spi':spi_state).
 (ref_rel ds_abs1 dr spi) /\ (local_tr (dr, spi) lbl (dr', spi')) ==>
 (lbl <> tau ==> ?ds_abs1'. (ds_abs1_tr ds_abs1 lbl ds_abs1') /\ (ref_rel ds_abs1' dr' spi'))``,
 rw [local_tr_cases] >|
@@ -29,7 +29,7 @@ METIS_TAC [abs1_comb_hold_ref_rel_XFER]]);
 
 (* simulation: ds_abs1 or ds_abs1' exists for ref_rel holding when lbl is tau *)
 val abs1_comb_hold_ref_rel_tau = store_thm("abs1_comb_hold_ref_rel_tau",
-``!(spi:spi_state) (dr:driver_state) (ds_abs1:ds_abs1_state).
+``!(spi:spi_state) (dr:driver_state) (ds_abs1:ds_abs1_state) (dr':driver_state) (spi':spi_state).
 (ref_rel ds_abs1 dr spi) /\ (local_tr (dr, spi) tau (dr', spi')) ==>
 (ref_rel ds_abs1 dr' spi') \/ (?ds_abs1'. (ds_abs1_tr ds_abs1 tau ds_abs1') /\ (ref_rel ds_abs1' dr' spi'))``,
 rw [local_tr_cases] >|
@@ -38,18 +38,21 @@ METIS_TAC [abs1_comb_hold_ref_rel_spi_tr],
 METIS_TAC [abs1_comb_hold_ref_rel_WR_UP],
 METIS_TAC [abs1_comb_hold_ref_rel_RD_RE]]);
 
-(* simulation: ds_abs1' or ds_abs1 for ref_rel holding  *)
+(* simulation: when (dr, spi) performs state transition, ds_abs1 is simulated to (dr,spi). *)
 val abs1_comb_hold_ref_rel = store_thm("abs1_comb_hold_ref_rel",
-``!(spi:spi_state) (dr:driver_state) (ds_abs1:ds_abs1_state) (lbl:global_lbl_type).
+``!(spi:spi_state) (dr:driver_state) (ds_abs1:ds_abs1_state) (lbl:global_lbl_type) (dr':driver_state) (spi':spi_state).
 (ref_rel ds_abs1 dr spi) /\ (local_tr (dr, spi) lbl (dr', spi')) ==>
-(lbl <> tau ==> ?ds_abs1'. (ds_abs1_tr ds_abs1 lbl ds_abs1') /\ (ref_rel ds_abs1' dr' spi')) /\
-(lbl = tau ==> (ref_rel ds_abs1 dr' spi') \/ (?ds_abs1'. (ds_abs1_tr ds_abs1 tau ds_abs1') \/ (ref_rel ds_abs1' dr' spi')))``,
+(?ds_abs1'. (ds_abs1_tr ds_abs1 lbl ds_abs1') /\ (ref_rel ds_abs1' dr' spi')) \/
+(ref_rel ds_abs1 dr' spi')``,
 rw []  >>
+Cases_on `lbl = tau` >>
 METIS_TAC [abs1_comb_hold_ref_rel_tau, abs1_comb_hold_ref_rel_not_tau_lbl]);
 
+
+(* when ds_abs1 performs state transition, (dr,spi) is simulated to ds_abs1 *)
 (* simulation: (dr', spi') exists when lbl is not tau *)
 val comb_abs1_hold_ref_rel_not_tau_lbl = store_thm("comb_abs1_hold_ref_rel_not_tau_lbl",
-``!(spi:spi_state) (dr:driver_state) (ds_abs1:ds_abs1_state) (lbl:global_lbl_type).
+``!(spi:spi_state) (dr:driver_state) (ds_abs1:ds_abs1_state) (lbl:global_lbl_type) (ds_abs1':ds_abs1_state).
 (ref_rel ds_abs1 dr spi) /\ (ds_abs1_tr ds_abs1 lbl ds_abs1') ==>
 (lbl <> tau ==> ?dr' spi'. (local_tr (dr, spi) lbl (dr', spi')) /\ (ref_rel ds_abs1' dr' spi'))``,
 rw [ds_abs1_tr_cases] >|
@@ -63,7 +66,8 @@ rw [comb_abs1_hold_ref_rel_RX],
 rw [comb_abs1_hold_ref_rel_XFER]]);
 
 
-(* 
+(*
+
 val comb_abs1_hold_ref_rel_tau_spi = store_thm("comb_abs1_hold_ref_rel_tau_spi",
 ``!(spi:spi_state) (dr:driver_state) (ds_abs1:ds_abs1_state).
 (ref_rel ds_abs1 dr spi) /\ (ds_abs1_spi_tr ds_abs1 tau_spi ds_abs1') ==>
@@ -82,7 +86,6 @@ val comb_abs1_hold_ref_rel_tau_comb = store_thm("comb_abs1_hold_ref_rel_tau_comb
 ?dr' spi'. (local_tr (dr, spi) tau (dr', spi')) /\ (ref_rel ds_abs1' dr' spi')``,
 cheat);
 
-bi-simulation (dr',spi') when lbl is tau 
 val comb_abs1_hold_ref_rel_tau = store_thm("comb_abs1_hold_ref_rel_tau",
 ``!(spi:spi_state) (dr:driver_state) (ds_abs1:ds_abs1_state).
 (ref_rel ds_abs1 dr spi) /\ (ds_abs1_tr ds_abs1 tau ds_abs1') ==>
@@ -92,7 +95,6 @@ rw [ds_abs1_tr_cases] >|
 METIS_TAC [comb_abs1_hold_ref_rel_tau_dr],
 METIS_TAC [comb_abs1_hold_ref_rel_tau_comb]]);
 
-(* bi-simulation (dr, spi') *)
 val comb_abs1_hold_ref_rel = store_thm("comb_abs1_hold_ref_rel",
 ``!(spi:spi_state) (dr:driver_state) (ds_abs1:ds_abs1_state) (lbl:global_lbl_type).
 (ref_rel ds_abs1 dr spi) /\ (ds_abs1_tr ds_abs1 lbl ds_abs1') ==>
