ds_abs0/abs_relScript.sml
@@ -54,17 +54,47 @@ abs_rel (ds_abs0:ds_abs0_state) (ds_abs1:ds_abs1_state) =
 ((ds_abs0.err = ds_abs1.err) /\
 (IS_ABS_STATE_REL ds_abs0 ds_abs1) /\
 (ds_abs0.ds_abs0_tx.tx_data_buffer = ds_abs1.ds_abs1_tx.tx_data_buffer) /\
-(ds_abs0.ds_abs0_tx.tx_cur_length = ds_abs1.ds_abs1_tx.tx_cur_length) /\
+(* tx_cur_length depends on the state *)
+( ds_abs1.state = abs1_tx_idle \/ ds_abs1.state = abs1_tx_trans \/ ds_abs1.state = abs1_tx_reset ==>
+ds_abs0.ds_abs0_tx.tx_cur_length = ds_abs1.ds_abs1_tx.tx_cur_length) /\
+(ds_abs1.state = abs1_tx_done_1 \/ ds_abs1.state = abs1_tx_data_1 \/
+ds_abs1.state = abs1_tx_done_2 \/ ds_abs1.state = abs1_tx_data_2 \/
+ds_abs1.state = abs1_tx_update \/ ds_abs1.state = abs1_tx_last_update ==> 
+ds_abs1.ds_abs1_tx.tx_cur_length = ds_abs0.ds_abs0_tx.tx_cur_length + 1) /\
+(ds_abs1.state = abs1_tx_next \/ ds_abs1.state = abs1_tx_last ==>
+ds_abs1.ds_abs1_tx.tx_cur_length = ds_abs0.ds_abs0_tx.tx_cur_length + 2) /\
 (ds_abs0.ds_abs0_rx.rx_data_buffer = ds_abs1.ds_abs1_rx.rx_data_buffer) /\
 (ds_abs0.ds_abs0_rx.rx_left_length = ds_abs1.ds_abs1_rx.rx_left_length) /\
 (ds_abs0.ds_abs0_xfer.xfer_dataIN_buffer = ds_abs1.ds_abs1_xfer.xfer_dataIN_buffer) /\
 (ds_abs0.ds_abs0_xfer.xfer_dataOUT_buffer = ds_abs1.ds_abs1_xfer.xfer_dataOUT_buffer) /\
-(ds_abs0.ds_abs0_xfer.xfer_cur_length = ds_abs1.ds_abs1_xfer.xfer_cur_length) /\
+(ds_abs1.state <> abs1_xfer_data /\ ds_abs1.state <> abs1_xfer_exchange ==>
+ds_abs0.ds_abs0_xfer.xfer_cur_length = ds_abs1.ds_abs1_xfer.xfer_cur_length) /\
+(ds_abs1.state = abs1_xfer_data \/ ds_abs1.state = abs1_xfer_exchange ==>
+ds_abs1.ds_abs1_xfer.xfer_cur_length = ds_abs0.ds_abs0_xfer.xfer_cur_length + 1) /\
+(* rules for tx automaton *)
+(ds_abs1.state = abs1_tx_done_1 \/ ds_abs1.state = abs1_tx_data_1 \/ 
+ds_abs1.state = abs1_tx_last_update ==>
+~ (ds_abs1.ds_abs1_tx.tx_cur_length < LENGTH ds_abs1.ds_abs1_tx.tx_data_buffer)) /\
+(ds_abs1.state = abs1_tx_done_2 \/ ds_abs1.state = abs1_tx_data_2 \/
+ds_abs1.state = abs1_tx_update \/ ds_abs1.state = abs1_tx_next ==>
+ds_abs1.ds_abs1_tx.tx_cur_length < LENGTH ds_abs1.ds_abs1_tx.tx_data_buffer) /\
+(ds_abs1.state = abs1_tx_last ==>
+ds_abs1.ds_abs1_tx.tx_cur_length = LENGTH ds_abs1.ds_abs1_tx.tx_data_buffer) /\
+(ds_abs1.state = abs1_tx_last \/ ds_abs1.state = abs1_tx_next ==>
+ds_abs1.spi_abs1.TX_SHIFT_REG =
+EL (ds_abs1.ds_abs1_tx.tx_cur_length - 2) (ds_abs1.ds_abs1_tx.tx_data_buffer)) /\
+(ds_abs1.state = abs1_tx_done_1 \/ ds_abs1.state = abs1_tx_done_2 ==>
+ds_abs1.spi_abs1.TX_SHIFT_REG = 
+EL (ds_abs1.ds_abs1_tx.tx_cur_length - 1) (ds_abs1.ds_abs1_tx.tx_data_buffer)) /\
 (* some requirements for rx automaton *)
 (ds_abs0.state = abs0_rx_reading ==> ds_abs1.spi_abs1.RX_SHIFT_REG = ds_abs0.ds_abs0_rx.temp_RSR) /\
 (ds_abs0.state = abs0_rx_update ==> ds_abs1.spi_abs1.RX_SHIFT_REG = ds_abs0.ds_abs0_rx.temp_RSR) /\
 (ds_abs0.state = abs0_rx_next ==> ds_abs1.spi_abs1.RX_SHIFT_REG = ds_abs0.ds_abs0_rx.temp_RSR) /\
 (ds_abs0.state = abs0_rx_next ==> ds_abs1.ds_abs1_rx.temp_value = ds_abs0.ds_abs0_rx.temp_value) /\
-(ds_abs0.state = abs0_xfer_done ==> ds_abs1.spi_abs1.RX_SHIFT_REG = ds_abs0.ds_abs0_xfer.xfer_RSR))`
+(ds_abs1.state = abs1_rx_fetch_data ==> ds_abs1.ds_abs1_rx.temp_value = ds_abs1.spi_abs1.RX_SHIFT_REG) /\
+(* some requirements for xfer automaton *)
+(ds_abs0.state = abs0_xfer_done ==> ds_abs1.spi_abs1.RX_SHIFT_REG = ds_abs0.ds_abs0_xfer.xfer_RSR) /\
+(ds_abs1.state = abs1_xfer_exchange ==> ds_abs1.spi_abs1.TX_SHIFT_REG = 
+EL (ds_abs1.ds_abs1_xfer.xfer_cur_length - 1) (ds_abs1.ds_abs1_xfer.xfer_dataOUT_buffer)))`
 
 val _ = export_theory();
