spi_model/weak_bisimulationScript.sml
@@ -1,0 +1,25 @@
+open HolKernel bossLib boolLib Parse;
+open SPI_stateTheory;
+
+val _ = new_theory "weak_bisimulation";
+
+(* A state can be reached after n tau steps *)
+val n_tau_tr_def = Define `
+(n_tau_tr (0:num) (tr:'a -> global_lbl_type -> 'a -> bool) (s:'a) (lbl:global_lbl_type) (s':'a) = (tr s lbl s')) /\
+(n_tau_tr (n:num) (tr:'a -> global_lbl_type -> 'a -> bool) (s:'a) (lbl:global_lbl_type) (s':'a) = ?(s'':'a). (tr s tau s'') /\ (n_tau_tr (n-1) tr s'' lbl s'))`
+
+(* define the weak transition relation *)
+val weak_tr_def = Define `
+weak_tr (tr:'a -> global_lbl_type -> 'a -> bool) (s:'a) (lbl:global_lbl_type) (s':'a) = 
+((tr s lbl s') \/
+(s = s' /\ lbl = tau) \/
+(?n. n_tau_tr n tr s lbl s'))`
+
+(* define the weak bisimulation realtion *)
+val weak_bisim_def = Define `
+weak_bisim (r:'a -> 'b -> bool) (tr1:'a -> global_lbl_type -> 'a -> bool) (tr2:'b -> global_lbl_type -> 'b -> bool) =
+(!s1 s2. r s1 s2 ==>
+(!lbl s1'. tr1 s1 lbl s1' ==> ?s2'. weak_tr tr2 s2 lbl s2' /\ r s1' s2') /\
+(!lbl s2'. tr2 s2 lbl s2' ==> ?s1'. weak_tr tr1 s1 lbl s1' /\ r s1' s2'))`
+
+val _ = export_theory();
